removal of top in progress

theories/SLFAffine.v
@@ -32,3 +32,561 @@ Implicit Types Q : val->hprop.
 (** ** Notion of weakest precondition *)
 
 
+
+(** The "top" heap predicate, written [\Top], holds of any heap predicate.
+    It plays a useful role for denoting pieces of state that needs to be
+    discarded, reflecting in the logic the action of the garbage collector. *)
+
+Definition htop : hprop :=
+  fun (h:heap) => True.
+
+Notation "\Top" := (htop).
+
+
+
+Lemma htop_intro : forall h,
+  \Top h.
+Proof using. intros. hnf. auto. Qed.
+
+
+Lemma htop_inv : forall h, (* Note: this lemma is of no practical interest. *)
+  \Top h ->
+  True.
+Proof using. intros. auto. Qed.
+
+
+
+(* ******************************************************* *)
+(** ** Separation Logic triples and the garbage collection rule *)
+
+(** To conduct verification proofs in a language equipped with a garbage
+    collector, we need to be able to discard pieces of states when they
+    become useless. Concretely, we need the rule shown below to hold.
+    The [\Top] predicate captures any (un)desired piece of state. *)
+
+Parameter triple_htop_post' : forall t H Q,
+  triple t H (Q \*+ \Top) ->
+  triple t H Q.
+
+(** Above, recall that [\Top] is defined as [fun h => True]. Thus, for 
+    some value [v], the heap predicate [(Q \*+ \Top) v] holds of any state
+    that decomposes as a disjoint union of the form [h1 \u h2], such that
+    [Q v h1] holds. In other words, [(Q \*+ \Top) v] holds of any state
+    that contains a sub-state [h1] such that [Q v h1] holds. *)
+
+(** The definition [triple1] provided earlier does not allow deriving the
+    rule [triple_htop_post']. However, we can tweak slightly the definition
+    to enable it. Concretely, in the definition of [triple1], we augment the 
+    postcondition of the underlying Hoare triple with an extra [\Top].
+    Intuitively, this added [\Top] captures any piece of state that we do not 
+    wish to mention explicitly in the postcondition.
+
+    The updated definition, called [triple], is as follows. *)
+
+Definition triple (t:trm) (H:hprop) (Q:val->hprop) : Prop :=
+  forall (H':hprop), hoare t (H \* H') (Q \*+ H' \*+ \Top).
+
+(** From there, we can prove that the desired rule for discarding pieces 
+    of postconditions holds. We can also prove that the frame rule still holds
+    for the modified definition. The proof of these two results is studied further. *)
+
+Parameter triple_htop_post : forall t H Q,
+  triple t H (Q \*+ \Top) ->
+  triple t H Q.
+
+Parameter triple_frame : forall t H Q H',
+  triple t H Q ->
+  triple t (H \* H') (Q \*+ H').
+
+(** Remark: it may also be useful to set up finer-grained versions of Separation Logic, 
+    where only certain types of heap predicates  can be discarded, but not all. Technically, 
+    only "affine" predicates may be discarded. Such a set up is discussed in the chapter
+    [SLFRich.v]. *)
+
+
+
+(** The top heap predicate [\Top] is equivalent to [\exists H, H],
+    which is a heap predicate that also characterizes any state.
+    Again, because we need [hexists] anyway, we prefer in practice
+    to define [\Top] in terms of [hexists], as done in the definition
+    of [htop'] shown below. *)
+
+Lemma htop_eq_hexists_hprop :
+  \Top = (\exists (H:hprop), H).
+Proof using.
+  unfold htop, hexists. apply hprop_eq. intros h. iff Hh.
+  { exists (=h). auto. }
+  { auto. }
+Qed.
+
+Definition htop' : hprop :=
+  \exists (H:hprop), H.
+
+(** In summary, in subsequent chapters, we assume the following definitions:
+
+[[
+
+  Definition htop : hprop :=
+    \exists (H:hprop), H.
+]]
+*)
+
+
+
+
+(* ******************************************************* *)
+(** ** Establishing properties of [triple]: exercises. *)
+
+(* EX1! (triple_frame) *)
+(** Prove the frame rule for the actual definition of [triple].
+    Take inspiration from the proof of [SL_frame_rule]. *)
+
+Lemma triple_frame' : forall t H Q H',
+  triple t H Q ->
+  triple t (H \* H') (Q \*+ H').
+Proof using.
+(* SOLUTION *)
+  introv M. unfold triple in *. rename H' into H1. intros H2.
+  specializes M (H1 \* H2). applys_eq M 1 2.
+  { rewrite hstar_assoc. auto. }
+  { applys qprop_eq. intros v.
+    repeat rewrite hstar_assoc. auto. }
+(* /SOLUTION *)
+Qed.
+
+(** The other main property to establish is [triple_htop_post].
+
+    The proof expoits associativity and commutativity of the star
+    operator, as well as a property asserting that [\Top \* \Top]
+    simplifies to [\Top]: both heap predicate can be used
+    to describe arbitrary heaps. These properties are assumed here;
+    they are proved in the next chapter ([SLFHimpl]). *)
+
+Parameter hstar_assoc' : forall H1 H2 H3,
+  (H1 \* H2) \* H3 = H1 \* (H2 \* H3).
+
+Parameter hstar_comm : forall H1 H2,
+  H1 \* H2 = H2 \* H1.
+
+Parameter hstar_htop_htop :
+  \Top \* \Top = \Top.
+
+(* EX3! (triple_htop_post'') *)
+(** Prove lemma [triple_htop_post], by unfolding the definition of [triple]
+    to reveal [hoare]. Note, however, that your proof should not attempt to
+    unfold the definition of a [hoare] triple. *)
+
+Lemma triple_htop_post'' : forall t H Q,
+  triple t H (Q \*+ \Top) ->
+  triple t H Q.
+Proof using.
+(* SOLUTION *)
+  introv M. unfold triple in *. intros H2.
+  specializes M H2. applys_eq M 1.
+  { applys qprop_eq. intros v. repeat rewrite hstar_assoc.
+    rewrite (hstar_comm H2).
+    rewrite <- (hstar_assoc \Top \Top).
+    rewrite hstar_htop_htop. auto. }
+(* /SOLUTION *)
+Qed.
+
+
+
+(** Recall the final definition of [triple], as:
+    [forall (H':hprop), hoare (H \* H') t (Q \*+ H' \*+ \Top)].
+
+    This definition can also be reformulated directly in terms of union
+    of heaps. All we need to do is introduce an additional piece of
+    state to describe the part covered by new [\Top] predicate.
+
+    In order to describe disjointness of the 3 pieces of heap that
+    describe the final state, we first introduce an auxiliary definition:
+    [Fmap.disjoint_3 h1 h2 h3] asserts that the three arguments denote
+    pairwise disjoint heaps. *)
+
+Definition fmap_disjoint_3 (h1 h2 h3:heap) : Prop :=
+     Fmap.disjoint h1 h2
+  /\ Fmap.disjoint h2 h3
+  /\ Fmap.disjoint h1 h3.
+
+(** We then generalize the result heap from [h1' \u h2] to
+    [h1' \u h2 \u h3'], where [h3'] denotes the piece of the
+    final state that is described by the [\Top] heap predicate
+    that appears in the definition of [triple]. *)
+
+Definition triple_lowlevel (t:trm) (H:hprop) (Q:val->hprop) : Prop :=
+  forall h1 h2,
+  Fmap.disjoint h1 h2 ->
+  H h1 ->
+  exists v h1' h3',
+       fmap_disjoint_3 h1' h2 h3'
+    /\ eval (h1 \u h2) t (h1' \u h2 \u h3') v
+    /\ Q v h1'.
+
+(** One can prove the equivalence of [triple] and [triple_lowlevel]
+    following a similar proof pattern as previously. The proof is a bit
+    more technical and requires additional tactic support to deal with
+    the tedious disjointness conditions, so we omit the details here. *)
+
+Parameter triple_iff_triple_lowlevel : forall t H Q,
+  triple t H Q <-> triple_lowlevel t H Q.
+
+(* INSTRUCTORS *)
+(** The proof of the above lemma is included in the file [SepBase.v] from CFML2. *)
+(* /INSTRUCTORS *)
+
+
+
+(* ******************************************************* *)
+(** ** The [xsimpl] tactic *)
+
+    4. Eliminate any redundant [\Top] from the RHS.
+
+
+(** Finally, [xsimpl] provides support for eliminating [\Top] on the RHS.
+    First, if the RHS includes several occurences of [\Top], then they
+    are replaced with a single one. *)
+
+Lemma xsimpl_demo_rhs_htop_compact : forall H1 H2 H3 H4,
+  H1 \* H2 ==> H3 \* \Top \* H4 \* \Top.
+Proof using.
+  intros. xsimpl.
+Abort.
+
+(** Second, if after cancellations the RHS consists of exactly
+   [\Top] and nothing else, then the goal is discharged. *)
+
+Lemma xsimpl_demo_rhs_htop : forall H1 H2 H3,
+  H1 \* H2 \* H3 ==> H3 \* \Top \* H2 \* \Top.
+Proof using.
+  intros. xsimpl.
+Abort.
+
+
+
+Lemma himpl_example_3 : forall (p q:loc),
+  p ~~~> 3 \* q ~~~> 3 ==>
+  p ~~~> 3 \* \Top.
+Proof using. xsimpl. Qed.
+
+
+   Note: [q ~~~> 4 \* p ~~~> 3 ==> p ~~~> 3 \* \Top] would be true.
+
+
+(* ******************************************************* *)
+(** ** Combined structural rules *)
+
+
+(** The "combined structural rule" generalizes the rule above
+    by also integrating the garbage collection rule. *)
+
+Lemma triple_conseq_frame_htop : forall H2 H1 Q1 t H Q,
+  triple t H1 Q1 ->
+  H ==> H1 \* H2 ->
+  Q1 \*+ H2 ===> Q \*+ \Top ->
+  triple t H Q.
+
+(* EX1! (triple_conseq_frame_htop) *)
+(** Prove the combined structural rule. 
+    Hint: recall lemma [triple_htop_post]. *)
+
+Proof using.
+(* SOLUTION *)
+  introv M WH WQ. applys triple_htop_post.
+  applys~ triple_conseq_frame M WH WQ.
+(* /SOLUTION *)
+Qed.
+
+
+
+
+
+(* ******************************************************* *)
+(** ** Entailment lemmas for [\Top] *)
+
+(* EX1! (himpl_htop_r) *)
+(** Prove that any heap predicate entails [\Top] *)
+
+Lemma himpl_htop_r : forall H,
+  H ==> \Top.
+Proof using.
+(* SOLUTION *)
+  intros. intros h Hh.
+  applys htop_intro. (* hnf; auto. *)
+(* /SOLUTION *)
+Qed.
+
+(* EX2! (hstar_htop_htop) *)
+(** Prove that [\Top \* \Top] is equivalent to [\Top] *)
+
+Lemma hstar_htop_htop :
+  \Top \* \Top = \Top.
+Proof using.
+(* SOLUTION *)
+  applys himpl_antisym.
+  { applys himpl_htop_r. }
+  { rewrite <- hstar_hempty_l at 1. applys himpl_frame_l.
+    applys himpl_htop_r. }
+(* /SOLUTION *)
+Qed.
+
+
+
+(* ******************************************************* *)
+(** ** Variants for the garbage collection rule *)
+
+(** Recall the lemma [triple_htop_post] from the previous chapter. *)
+
+Parameter triple_htop_post : forall t H Q,
+  triple t H (Q \*+ \Top) ->
+  triple t H Q.
+
+(* EX2! (triple_hany_post) *)
+(** The following lemma provides an alternative presentation of the
+    same result as [triple_htop_post]. Prove that it is derivable
+    from [triple_htop_post] and [triple_conseq]. *)
+
+Lemma triple_hany_post : forall t H H' Q,
+  triple t H (Q \*+ H') ->
+  triple t H Q.
+Proof using.
+(* SOLUTION *)
+  introv M. applys* triple_htop_post. applys triple_conseq M.
+  { applys himpl_refl. }
+  { intros v. applys himpl_frame_r. applys himpl_htop_r. }
+(* /SOLUTION *)
+Qed.
+
+(** Reciprocally, [triple_htop_post] is trivially derivable from
+    [triple_hany_post], simply by instantiating [H'] as [\Top]. *)
+
+Lemma triple_htop_post_derived_from_triple_hany_post : forall t H Q,
+  triple t H (Q \*+ \Top) ->
+  triple t H Q.
+Proof using. intros. applys triple_hany_post \Top. auto. Qed.
+
+(** The reason we prefer [triple_htop_post] to [triple_hany_post]
+    is that it does not require providing [H'] at the time of applying
+    the rule. The instantiation is postponed through the introduction
+    of [\Top], which is equivalent to [\exists H', H']. Delaying the
+    instantiation of [H'] using [\Top] rather than throught the
+    introduction of an evar enables more robust proof scripts and
+    tactic support. *)
+
+(* EX2! (triple_htop_pre) *)
+(** The rule [triple_htop_post] enables discarding pieces of
+    heap from the postcondition. The symmetric rule [triple_htop_pre]
+    enables discarding pieces of heap from the precondition.
+
+    Prove that it is derivable from [triple_htop_post] and
+    [triple_frame] (and, optionally, [triple_conseq]). *)
+
+Lemma triple_htop_pre : forall t H Q,
+  triple t H Q ->
+  triple t (H \* \Top) Q.
+Proof using.
+(* SOLUTION *)
+  introv M. applys triple_htop_post. applys triple_frame. auto.
+(* /SOLUTION *)
+Qed.
+
+(* EX2! (triple_htop_pre) *)
+(** The rule [triple_hany_pre] is a variant of [triple_htop_pre].
+    Prove that it is derivable.
+    You may exploit [triple_htop_pre], or [triple_hany_post],
+    or [triple_htop_post], whichever you find simpler. *)
+
+Lemma triple_hany_pre : forall t H H' Q,
+  triple t H Q ->
+  triple t (H \* H') Q.
+Proof using.
+(* SOLUTION *)
+  dup 3.
+  (* first proof, based on [triple_hany_post]: *)
+  introv M. applys triple_hany_post. applys triple_frame. auto.
+  (* second proof, based on [triple_htop_pre]: *)
+  introv M. lets N: triple_htop_pre M. applys triple_conseq N.
+  { applys himpl_frame_r. applys himpl_htop_r. }
+  { applys qimpl_refl. }
+  (* third proof, based on [triple_htop_post]: *)
+  introv M. applys triple_htop_post.
+  lets N: triple_frame H' M.
+  applys triple_conseq N.
+  { applys himpl_refl. }
+  { intros v. applys himpl_frame_r. applys himpl_htop_r. }
+(* /SOLUTION *)
+Qed.
+
+(** Here again, the reciprocal holds: [triple_hany_pre] is trivially
+    derivable from [triple_htop_pre]. The variant of the rule that is
+    most useful in practice is actually yet another presentation,
+    which applies to any goal and enables specifying explicitly the
+    piece of the precondition that one wishes to discard. *)
+
+Lemma triple_hany_pre_trans : forall H1 H2 t H Q,
+  triple t H1 Q ->
+  H ==> H1 \* H2 ->
+  triple t H Q.
+Proof using.
+  introv M WH. applys triple_conseq (H1 \* H2) Q.
+  { applys triple_hany_pre. auto. }
+  { applys WH. }
+  { applys qimpl_refl. }
+Qed.
+
+(** Remark: the lemmas that enable discarding pieces of precondition
+    (e.g., [triple_htop_pre]) are derivable from those that enable
+    discarding pices of postconditions (e.g., [triple_htop_post]),
+    but not the other way around.
+
+    Advanced remark: the above remark can be mitigated. If we expose
+    that [triple t H Q <-> triple t' H Q] holds whenever [t] and [t']
+    are observationally equivalent with respect to the semantics
+    defined by [eval], and if we are able to prove that [let x = t in x]
+    is observationally equivalent to [t] for some fresh variable x,
+    then it is possible to prove that [triple_htop_post] is derivable
+    from [triple_htop_pre]. Indeed, the postcondition of [t] can be viewed 
+    as the precondition of the [x] occuring in the right-hand side of the 
+    term [let x = t in x]. Thus, discarding a heap predicate from the
+    postcondition of [t] can be simulated by discarding a heap predicate
+    from the precondition of [x]. *)
+
+
+
+
+(* ******************************************************* *)
+(** ** Strucutral rules *)
+
+
+(** The garbage collection rules enable to discard any desired
+    piece of heap from the precondition or the postcondition.
+    Recall that the first rule is derivable from the second one.
+    Moreover, it is equivalent to state these two rules by writing 
+    [H'] instead of [\Top]. *)
+
+Parameter triple_htop_pre : forall t H Q,
+  triple t H Q ->
+  triple t (H \* \Top) Q.
+
+Parameter triple_htop_post : forall t H Q,
+  triple t H (Q \*+ \Top) ->
+  triple t H Q.
+
+
+
+
+
+(** Recall from the previous chapter the combined structural
+    rule [triple_conseq_frame_htop], which generalizes the rule
+    [triple_conseq_frame] with the possibility to discard
+    undesired heap predicate. This rule will be handy at
+    some point in the exercise that follows. *)
+
+Parameter triple_conseq_frame_htop : forall H2 H1 Q1 t H Q,
+  triple t H1 Q1 ->
+  H ==> H1 \* H2 ->
+  Q1 \*+ H2 ===> Q \*+ \Top ->
+  triple t H Q.
+
+
+
+
+Lemma triple_seq : forall t1 t2 H Q H1,
+  triple t1 H (fun v => H1) ->
+  triple t2 H1 Q ->
+  triple (trm_seq t1 t2) H Q.
+Proof using.
+  (* 1. We unfold the definition of [triple] to reveal a [hoare] judgment. *)
+  introv M1 M2. intros H'. (* optional: *) unfolds triple.
+  (* 2. We invoke the reasoning rule [hoare_seq] that we have just established. *)
+  applys hoare_seq.
+  { (* 3. For the hypothesis on the first subterm [t1],
+       we can invoke directly our first hypothesis. *)
+    applys M1. }
+    ...
+  { (* 4. For the hypothesis on the first subterm [t2],
+       we need a little more work to exploit our second hypothesis.
+       Indeed, the precondition features an extra [\Top].
+       To handle it, we need to instantiate [M2] with [H' \* \Top],
+       then merge the two [\Top] that appear into a single one.
+       We could begin the proof script with:
+         [specializes M2 (H' \* \Top). rewrite <- hstar_assoc in M2.]
+       However, it is simpler to directly invoke the consequence rule,
+       and let [xsimpl] do all the tedious work for us. *)
+    applys hoare_conseq. { applys M2. } { xsimpl. } { xsimpl. } }
+Qed.
+
+
+
+
+
+
+(** [wp] is defined on top of [hoare] triples. More precisely [wp t Q]
+    is a heap predicate such that [H ==> wp t Q] if and
+    only if [SL_triple t H Q], where [SL_triple t H Q]
+    is defined as [forall H', hoare t (H \* H') (Q \*+ H' \*+ \Top)]. *)
+
+Definition wp (t:trm) := fun (Q:val->hprop) =>
+  \exists H, H \* \[forall H', hoare t (H \* H') (Q \*+ H' \*+ \Top)].
+
+
+
+Lemma wp_ramified : forall Q1 Q2 t,
+  (wp t Q1) \* (Q1 \--* Q2 \*+ \Top) ==> (wp t Q2).
+Proof using.
+  intros. unfold wp. xpull ;=> H M.
+  xsimpl (H \* (Q1 \--* Q2 \*+ \Top)). intros H'.
+  applys hoare_conseq M; xsimpl.
+Qed.
+
+
+Lemma wp_hany_pre : forall t H Q,
+  (wp t Q) \* H ==> wp t Q.
+Proof using. intros. applys himpl_trans_r wp_ramified. xsimpl. Qed.
+
+Lemma wp_hany_post : forall t H Q ,
+  wp t (Q \*+ H) ==> wp t Q.
+Proof using. intros. applys himpl_trans_r wp_ramified. xsimpl. Qed.
+
+
+Definition triple (t:trm) (H:hprop) (Q:val->hprop) : Prop :=
+  forall (H':hprop), hoare t (H \* H') (Q \*+ H' \*+ \Top).
+
+
+Definition mkstruct (F:formula) : formula :=
+  fun Q => \exists Q', F Q' \* (Q' \--* (Q \*+ \Top)).
+
+
+Lemma mkstruct_ramified : forall Q1 Q2 F,
+  (mkstruct F Q1) \* (Q1 \--* Q2 \*+ \Top) ==> (mkstruct F Q2).
+Proof using. unfold mkstruct. xsimpl. Qed.
+
+
+
+
+Lemma xcf_lemma_fun : forall v1 v2 x t H Q,
+  v1 = val_fun x t ->
+  H ==> wpgen ((x,v2)::nil) t (Q \*+ \Top) ->
+  triple (trm_app v1 v2) H Q.
+Proof using.
+  introv M1 M2. rewrite wp_equiv.
+  applys himpl_trans; [| applys (>> wp_hany_post \Top)].
+  xchange M2.
+  xchange (>> wpgen_sound ((x,v2)::nil) t (Q \*+ \Top)).
+  rewrite <- subst_eq_isubst_one. applys* wp_app_fun.
+Qed.
+
+Lemma xcf_lemma_fix : forall v1 v2 f x t H Q,
+  v1 = val_fix f x t ->
+  H ==> wpgen ((f,v1)::(x,v2)::nil) t (Q \*+ \Top) ->
+  triple (trm_app v1 v2) H Q.
+Proof using.
+  introv M1 M2. rewrite wp_equiv. xchange M2.
+  applys himpl_trans; [| applys (>> wp_hany_post \Top)].
+  xchange (>> wpgen_sound (((f,v1)::nil) ++ (x,v2)::nil) t (Q \*+ \Top)).
+  rewrite isubst_app. do 2 rewrite <- subst_eq_isubst_one.
+  applys* wp_app_fix.
+Qed.
+
+
+
